\documentclass[12pt]{article}
\usepackage{amsmath}
\usepackage[hmargin=1in,vmargin=1in]{geometry}
\usepackage{amsfonts}
\usepackage{amssymb}
\usepackage{fancyhdr}
\usepackage{lastpage}
\usepackage{parskip} % Kill first paragraph indenting
\usepackage{tikz}
\usepackage[T1]{fontenc}
\usepackage{environ}



\pagestyle{fancy}
\fancyhead[L]{Omeed Mariani \\ CMSC/Math 207}
\fancyhead[R]{HW 7 \\ Page \thepage\ of \pageref{LastPage}}

\newcounter{problemnum}
\newcommand{\newprob}{\addtocounter{problemnum}{1} \noindent (\textbf{\arabic{problemnum}) }}

\begin{document}

\newprob
For $n \in \mathbb{N}$, let $P(n)$ be the predicate $\sum_{k=1}^{n-1}$ $k(k+1)$ = $\frac{n(n-1)(n+1)}{3}$.
Show for all $n \geq 2$:
\begin{align*}
LHS
&=1(1+1)=2.\\
RHS
&=\frac{2(2-1)(2+1)}{3}\\
&=2.
\end{align*}
\therefore $P(1)$ \text{is true}.\\
\textbf{Inductive Hypothesis}\\
\text{Assume for some arbitrary } n $  \geq 2$ that $P(n)$, that is $\sum_{k=1}^{n-1}$ $k(k+1)$ = $\frac{n(n-1)(n+1)}{3}$ holds.\\
\textbf{Inductive Step:}\\

\begin{align*}
\sum_{k=1}^{n} k(k+1)
&=\sum_{k=1}^{n-1} k(k+1)+n(n+1)\\
&=\frac{n(n-1)(n+1)}{3}+n(n+1)\\
&=\frac{n(n-1)(n+1)+3(n+1)n}{3}\\
&=\frac{(n+1)(n)(n-1+3)}{3}\\
&=\frac{n(n-1)(n+1)}{3}.
\end{align*}

Thus, $P(n+1)$ \text{ is true and so we have proved the inductive step.}\\
\text{Therefore by the principle of Mathmatical Induction, }$\sum_{k=1}^{n-1}$ $k(k+1)$ = $\frac{n(n-1)(n+1)}{3}$ \text { is true for all }$n \in \mathbb{N}$

\newprob

For $n \in \mathbb{N}$, let $P(n)$ be the predicate $\sum_{k=1}^{n+1}$ $k \cdot 2^k$ = $n \cdot 2^{n+2}+2$.\\
\text{Show for all } $n \geq 0$:
\begin{align*}
LHS
&=1*2^1=2,\\
RHS
&=0*2^{0+2}+2=2.\\
\end{align*}
\textbf{Inductive Hypothesis}\\
Assume for some arbitrary $n \geq 0$ that $P(n)$ that is $\sum_{k=1}^{n+1}$ $k \cdot 2^k$ = $n \cdot 2^{n+2}+2$ holds.\\
\textbf{Inductive Step:}\\
\begin{align*}
\sum_{k=1}^{n} k \cdot 2^k
&=\sum_{k=1}^{n+1} k \cdot 2^k + (n+2) \cdot 2^{n+2}\\
&=n \cdot 2^{n+2}+2+(n+2)\cdot 2^{n+2}\\
&=(2m+2) \cdot 2^{n+2}+2\\
&=2(n+1) \cdot 2^{n+2}+2\\
&=(n+1) \cdot 2^{n+2} +2
\end{align*}
Thus, $P(n+1)$ \text{ is true and so we have proved the inductive step.}\\
\text{Therefore by the principles of Mathmatical Induction } $\sum_{k=1}^{n+1}$
$k \cdot 2^k$ = $n \cdot 2^{n+2}+2$ \text { is true for all }$n \in \mathbb{N}$.






































\end{document}
