\documentclass[12pt]{article}
\usepackage{amsmath}
\usepackage[hmargin=1in,vmargin=1in]{geometry}
\usepackage{amsfonts}
\usepackage{amssymb}
\usepackage{fancyhdr}
\usepackage{lastpage}
\usepackage{parskip} % Kill first paragraph indenting
\usepackage{tikz}
\usepackage[T1]{fontenc}
\usepackage{environ}



\pagestyle{fancy}
\fancyhead[L]{Omeed Mariani \\ CMSC/Math 207}
\fancyhead[R]{HW 9 \\ Page \thepage\ of \pageref{LastPage}}

\newcounter{problemnum}
\newcommand{\newprob}{\addtocounter{problemnum}{1} \noindent (\textbf{\arabic{problemnum}) }}

\begin{document}

\newprob Use induction to prove that for all integers $n \geq 0$, $F_{n+2}F_n-F^2_{n+1}$ = $(-1)^n$.\\
\textbf{Basis of Induction}\\
For $n \in \mathbb{N}$, let $P(n)$ be the predicate $F_{n+2}F_n-F^2_{n+1}$ = $(-1)^n$.\\

\begin{align*}
&F_2F_0-F^2_1\\
&=1 \cdot 2-1^2\\
&=(-1)^0\\
\end{align*}\\
So $P(0)$ is true.\\
\textbf{Inductive Hypothesis}\\
Let  $F_{n+2}F_n-F^2_{n+1}$ = $(-1)^n$ be true for some $n \in \mathbb{W}$.\\
\textbf{Inductive Step}\\
\begin{align*}
&F_{n+3}F_{n+1}-F^2_{n+2}\\
&=F_{n+3}=F_{n+1}+F_{n+2}\\
&=(F_{n+1}+F_{n+2})F_{n+1}-F^2_{n+2}\\
&=F^2_{n+1}+F_{n+1}F_{n+2}-F^2_{n+2}\\
&=F^2_{n+2} = F_{n+2}F_n-(-1)^n\\
&=F_{n+2}F_n-(-1)^n+F_{n+1}F_{n+2}-F^2_{n+2}\\
&=F_{n+2}(F_n+F_{n+1})-(-1)^n-F^2_{n+2}\\
&=F_n+F_{n+1}=F_{n+2}\\
&=F^2_{n+2}-(-1)^n-F^2_{n+2}\\
&=-(-1)^n\\
&=(-1)^{n+1}.\\
\end{align*}
We finally have $F_{n+3}F_{n+1}-F^2_{n+2}=(-1)^{n+1}.$
\therefore $F_{n+2}F_n-F^2_{n+1}$ = $(-1)^n$







































\end{document}
